add make generate and organize instructions

examples/example.s
@@ -1,0 +1,24 @@
+test1:
+    bl fn1
+    mov x28, x0
+    str x28, [x27]
+    nop
+
+fn1:
+    mov w0, 0
+    ret
+
+test2:
+    cmp x1, 0
+    bne 0xc
+    mov x0, 1
+    b branch2
+branch1:
+    bl fn2
+branch2:
+    mov x28, x0
+    nop
+
+fn2:
+    mov x0, 0
+    ret
