examples/memory_instructions.s
@@ -1,0 +1,4 @@
+memory_instructions:
+    stp	x0, x1, [sp, #-16]!
+    ldr	x0, [x1]
+    str	x9, [x1]
