instructions/ad2800003.v
@@ -1,7 +1,0 @@
-From isla Require Import isla_lang.
-
-Definition ad2800003 : list trc := [
-  [
-    WriteReg "R3" [] (Val_Bits [BV{64%N} 0x0%Z]) Mk_annot
-  ]
-].
