instructions/example/a1c.v
@@ -1,0 +1,34 @@
+From isla Require Import isla_lang.
+
+Definition a1c : list trc := [
+  [
+    Smt (DeclareConst 27%Z (Ty_BitVec 1%N)) Mk_annot;
+    ReadReg "PSTATE" [Field "Z"] (Val_Struct [("Z", Val_Symbolic 27%Z)]) Mk_annot;
+    Smt (DefineConst 38%Z (Unop (Not) (Binop (Eq) (Val (Val_Symbolic 27%Z) Mk_annot) (Val (Val_Bits [BV{1%N} 0x1%Z]) Mk_annot) Mk_annot) Mk_annot)) Mk_annot;
+    Branch 0%Z "model/aarch64.sail 12137:4 - 12139:5" Mk_annot;
+    Smt (Assert (Val (Val_Symbolic 38%Z) Mk_annot)) Mk_annot;
+    Smt (DeclareConst 39%Z (Ty_BitVec 64%N)) Mk_annot;
+    ReadReg "_PC" [] (Val_Symbolic 39%Z) Mk_annot;
+    Smt (DefineConst 40%Z (Manyop (Bvmanyarith Bvadd) [Val (Val_Symbolic 39%Z) Mk_annot; Val (Val_Bits [BV{64%N} 0xc%Z]) Mk_annot] Mk_annot)) Mk_annot;
+    ReadReg "PSTATE" [Field "nRW"] (Val_Struct [("nRW", Val_Bits [BV{1%N} 0x0%Z])]) Mk_annot;
+    ReadReg "CFG_ID_AA64PFR0_EL1_EL0" [] (Val_Bits [BV{4%N} 0x1%Z]) Mk_annot;
+    ReadReg "CFG_ID_AA64PFR0_EL1_EL1" [] (Val_Bits [BV{4%N} 0x1%Z]) Mk_annot;
+    ReadReg "CFG_ID_AA64PFR0_EL1_EL2" [] (Val_Bits [BV{4%N} 0x1%Z]) Mk_annot;
+    ReadReg "CFG_ID_AA64PFR0_EL1_EL3" [] (Val_Bits [BV{4%N} 0x1%Z]) Mk_annot;
+    Smt (DefineConst 52%Z (Val (Val_Symbolic 40%Z) Mk_annot)) Mk_annot;
+    BranchAddress (Val_Symbolic 52%Z) Mk_annot;
+    Smt (DefineConst 53%Z (Val (Val_Symbolic 40%Z) Mk_annot)) Mk_annot;
+    ReadReg "PSTATE" [Field "EL"] (Val_Struct [("EL", Val_Bits [BV{2%N} 0x2%Z])]) Mk_annot;
+    ReadReg "SCR_EL3" [] (Val_Bits [BV{32%N} 0x0%Z]) Mk_annot;
+    ReadReg "TCR_EL2" [] (Val_Bits [BV{64%N} 0x0%Z]) Mk_annot;
+    WriteReg "_PC" [] (Val_Symbolic 53%Z) Mk_annot;
+    WriteReg "__PC_changed" [] (Val_Bool true) Mk_annot
+  ];
+  [
+    Smt (DeclareConst 27%Z (Ty_BitVec 1%N)) Mk_annot;
+    ReadReg "PSTATE" [Field "Z"] (Val_Struct [("Z", Val_Symbolic 27%Z)]) Mk_annot;
+    Smt (DefineConst 38%Z (Unop (Not) (Binop (Eq) (Val (Val_Symbolic 27%Z) Mk_annot) (Val (Val_Bits [BV{1%N} 0x1%Z]) Mk_annot) Mk_annot) Mk_annot)) Mk_annot;
+    Branch 0%Z "model/aarch64.sail 12137:4 - 12139:5" Mk_annot;
+    Smt (Assert (Unop (Not) (Val (Val_Symbolic 38%Z) Mk_annot) Mk_annot)) Mk_annot
+  ]
+].
