instructions/example/a34.v
@@ -1,0 +1,7 @@
+From isla Require Import isla_lang.
+
+Definition a34 : list trc := [
+  [
+    WriteReg "R0" [] (Val_Bits [BV{64%N} 0x0%Z]) Mk_annot
+  ]
+].
