instructions/example/instrs.v
@@ -1,0 +1,30 @@
+From isla Require Import isla_lang.
+Require Export isla.instructions.example.a0.
+Require Export isla.instructions.example.a4.
+Require Export isla.instructions.example.a8.
+Require Export isla.instructions.example.a10.
+Require Export isla.instructions.example.a14.
+Require Export isla.instructions.example.a18.
+Require Export isla.instructions.example.a1c.
+Require Export isla.instructions.example.a20.
+Require Export isla.instructions.example.a24.
+Require Export isla.instructions.example.a28.
+Require Export isla.instructions.example.a2c.
+Require Export isla.instructions.example.a34.
+Require Export isla.instructions.example.a38.
+
+Definition instr_map := [
+  (0x0%Z, a0 (* bl 10 <fn1> *));
+  (0x4%Z, a4 (* mov x28, x0 *));
+  (0x8%Z, a8 (* str x28, [x27] *));
+  (0x10%Z, a10 (* mov w0, #0x0 *));
+  (0x14%Z, a14 (* ret *));
+  (0x18%Z, a18 (* cmp x1, #0x0 *));
+  (0x1c%Z, a1c (* b.ne 28 <branch1> *));
+  (0x20%Z, a20 (* mov x0, #0x1 *));
+  (0x24%Z, a24 (* b 2c <branch2> *));
+  (0x28%Z, a28 (* bl 34 <fn2> *));
+  (0x2c%Z, a2c (* mov x28, x0 *));
+  (0x34%Z, a34 (* mov x0, #0x0 *));
+  (0x38%Z, a38 (* ret *))
+].
