instructions/memcpy/a8.v
@@ -1,0 +1,38 @@
+From isla Require Import isla_lang.
+
+Definition a8 : list trc := [
+  [
+    Smt (DeclareConst 6%Z (Ty_BitVec 1%N)) Mk_annot;
+    Smt (DeclareConst 29%Z (Ty_BitVec 64%N)) Mk_annot;
+    Smt (DeclareConst 30%Z (Ty_BitVec 64%N)) Mk_annot;
+    Smt (Assert (Binop (Eq) (Manyop (Bvmanyarith Bvand) [Manyop (Bvmanyarith Bvadd) [Val (Val_Symbolic 29%Z) Mk_annot; Val (Val_Symbolic 30%Z) Mk_annot] Mk_annot; Val (Val_Bits [BV{64%N} 0xfff0000000000007%Z]) Mk_annot] Mk_annot) (Val (Val_Bits [BV{64%N} 0x0%Z]) Mk_annot) Mk_annot)) Mk_annot;
+    ReadReg "R3" [] (Val_Symbolic 30%Z) Mk_annot;
+    ReadReg "R1" [] (Val_Symbolic 29%Z) Mk_annot;
+    Smt (DefineConst 103%Z (Manyop (Bvmanyarith Bvadd) [Val (Val_Symbolic 29%Z) Mk_annot; Val (Val_Symbolic 30%Z) Mk_annot] Mk_annot)) Mk_annot;
+    ReadReg "PSTATE" [Field "EL"] (Val_Struct [("EL", Val_Bits [BV{2%N} 0x2%Z])]) Mk_annot;
+    Smt (DefineConst 107%Z (Binop (Eq) (Val (Val_Symbolic 103%Z) Mk_annot) (Manyop (Bvmanyarith Bvand) [Val (Val_Symbolic 103%Z) Mk_annot; Val (Val_Bits [BV{64%N} 0xffffffffffffffff%Z]) Mk_annot] Mk_annot) Mk_annot)) Mk_annot;
+    ReadReg "SCTLR_EL2" [] (Val_Bits [BV{64%N} 0x4000002%Z]) Mk_annot;
+    Smt (Assert (Unop (Not) (Unop (Not) (Val (Val_Symbolic 107%Z) Mk_annot) Mk_annot) Mk_annot)) Mk_annot;
+    Smt (Assert (Unop (Not) (Unop (Not) (Val (Val_Symbolic 107%Z) Mk_annot) Mk_annot) Mk_annot)) Mk_annot;
+    Smt (Assert (Binop (Eq) (Val (Val_Symbolic 103%Z) Mk_annot) (Manyop (Bvmanyarith Bvand) [Val (Val_Symbolic 103%Z) Mk_annot; Val (Val_Bits [BV{64%N} 0xffffffffffffffff%Z]) Mk_annot] Mk_annot) Mk_annot)) Mk_annot;
+    ReadReg "CFG_ID_AA64PFR0_EL1_EL2" [] (Val_Bits [BV{4%N} 0x1%Z]) Mk_annot;
+    ReadReg "CFG_ID_AA64PFR0_EL1_EL3" [] (Val_Bits [BV{4%N} 0x1%Z]) Mk_annot;
+    ReadReg "PSTATE" [Field "nRW"] (Val_Struct [("nRW", Val_Bits [BV{1%N} 0x0%Z])]) Mk_annot;
+    ReadReg "CFG_ID_AA64PFR0_EL1_EL0" [] (Val_Bits [BV{4%N} 0x1%Z]) Mk_annot;
+    ReadReg "CFG_ID_AA64PFR0_EL1_EL1" [] (Val_Bits [BV{4%N} 0x1%Z]) Mk_annot;
+    ReadReg "SCR_EL3" [] (Val_Bits [BV{32%N} 0x0%Z]) Mk_annot;
+    ReadReg "TCR_EL2" [] (Val_Bits [BV{64%N} 0x0%Z]) Mk_annot;
+    Smt (Assert (Unop (Not) (Unop (Not) (Binop (Eq) (Unop (Extract 63%N 52%N) (Val (Val_Symbolic 103%Z) Mk_annot) Mk_annot) (Val (Val_Bits [BV{12%N} 0x0%Z]) Mk_annot) Mk_annot) Mk_annot) Mk_annot)) Mk_annot;
+    Smt (Assert (Unop (Not) (Unop (Not) (Val (Val_Symbolic 107%Z) Mk_annot) Mk_annot) Mk_annot)) Mk_annot;
+    ReadReg "PSTATE" [Field "D"] (Val_Struct [("D", Val_Symbolic 6%Z)]) Mk_annot;
+    ReadReg "OSLSR_EL1" [] (Val_Bits [BV{32%N} 0x0%Z]) Mk_annot;
+    ReadReg "OSDLR_EL1" [] (Val_Bits [BV{32%N} 0x0%Z]) Mk_annot;
+    ReadReg "EDSCR" [] (Val_Bits [BV{32%N} 0x0%Z]) Mk_annot;
+    Smt (DeclareConst 1293%Z (Ty_BitVec 56%N)) Mk_annot;
+    Smt (DefineConst 1302%Z (Unop (ZeroExtend 8%N) (Manyop Concat [Val (Val_Bits [BV{4%N} 0x0%Z]) Mk_annot; Unop (Extract 51%N 0%N) (Val (Val_Symbolic 103%Z) Mk_annot) Mk_annot] Mk_annot) Mk_annot)) Mk_annot;
+    Smt (DeclareConst 1303%Z (Ty_BitVec 8%N)) Mk_annot;
+    ReadMem (Val_Symbolic 1303%Z) (Val_Enum ((Mk_enum_id 7%nat), Mk_enum_ctor 0%nat)) (Val_Symbolic 1302%Z) 1%N None Mk_annot;
+    Smt (DefineConst 1307%Z (Manyop Concat [Val (Val_Bits [BV{32%N} 0x0%Z]) Mk_annot; Manyop Concat [Val (Val_Bits [BV{24%N} 0x0%Z]) Mk_annot; Val (Val_Symbolic 1303%Z) Mk_annot] Mk_annot] Mk_annot)) Mk_annot;
+    WriteReg "R4" [] (Val_Symbolic 1307%Z) Mk_annot
+  ]
+].
