Makefile
@@ -19,6 +19,22 @@ frontend/tests/%.v.expected: frontend/tests/%.isla
 promote: $(patsubst %.isla,%.v.expected,$(wildcard frontend/tests/*.isla))
 .PHONY: promote
 
+generate:
+	export PATH=$$PWD/bin:$$PATH; dune exec -- isla-coq examples/memory_instructions.dump -d -o instructions  -n "a{op}" --coqdir=isla.instructions
+	mv instructions/aa9bf07e0.isla instructions/stp.isla
+	mv instructions/aa9bf07e0.v instructions/stp.v
+	mv instructions/af9400020.isla instructions/load.isla
+	mv instructions/af9400020.v instructions/load.v
+	mv instructions/af9000029.isla instructions/store.isla
+	mv instructions/af9000029.v instructions/store.v
+	rm instructions/instrs.v
+	export PATH=$$PWD/bin:$$PATH; dune exec -- isla-coq examples/example.dump -d -o instructions/example  -n "a{addr}" --coqdir=isla.instructions.example
+	export PATH=$$PWD/bin:$$PATH; dune exec -- isla-coq examples/memcpy.dump -d -o instructions/memcpy  -n "a{addr}" --coqdir=isla.instructions.memcpy
+	export PATH=$$PWD/bin:$$PATH; dune exec -- isla-coq examples/binary_search.dump -d -o instructions/binary_search  -n "a{addr}" --coqdir=isla.instructions.binary_search
+	export PATH=$$PWD/bin:$$PATH; dune exec -- isla-coq pkvm_handler/pkvm_handler.dump
+.PHONY: generate
+
+
 clean:
 	@dune clean
 .PHONY: clean
